TCB/LazyList.v
@@ -93,6 +93,7 @@ Fixpoint ll_safe_drop {X} (n: nat) (ll: lazy_list X) :=
       end
   end.
 
+Recursive Extraction Nrect.
 
   (* to lib *)
 Lemma ll_safe_drop_nth {X}: forall n (ll: lazy_list X) ll',
